\documentclass[10pt,portrait]{article}
\usepackage{multicol}
\usepackage{calc}
\usepackage{ifthen}
\usepackage[portrait]{geometry}
\usepackage{hyperref}

% This sets page margins to .5 inch if using letter paper, and to 1cm
% if using A4 paper. (This probably isn't strictly necessary.)
% If using another size paper, use default 1cm margins.
\ifthenelse{\lengthtest { \paperwidth = 8.5in}}
	{ \geometry{top=.2in,left=.1in,right=.1in,bottom=.2in} }

% Turn off header and footer
\pagestyle{empty}

% Redefine section commands to use less space
\makeatletter
\renewcommand{\section}{\@startsection{section}{1}{0mm}%
                                {-1ex plus -.5ex minus -.2ex}%
                                {0.5ex plus .2ex}%x
                                {\normalfont\normalsize\bfseries}}
\renewcommand{\subsection}{\@startsection{subsection}{2}{0mm}%
                                {-1explus -.5ex minus -.2ex}%
                                {0.5ex plus .2ex}%
                                {\normalfont\small\bfseries}}
\renewcommand{\subsubsection}{\@startsection{subsubsection}{3}{0mm}%
                                {-1ex plus -.5ex minus -.2ex}%
                                {1ex plus .2ex}%
                                {\normalfont\small\bfseries}}
\makeatother

% Define BibTeX command
\def\BibTeX{{\rm B\kern-.05em{\sc i\kern-.025em b}\kern-.08em
    T\kern-.1667em\lower.7ex\hbox{E}\kern-.125emX}}

% Don't print section numbers
\setcounter{secnumdepth}{0}


\setlength{\parindent}{0pt}
\setlength{\parskip}{0pt plus 0.1ex}


% -----------------------------------------------------------------------

\begin{document}

\raggedright
\footnotesize
\begin{multicols}{2}


% multicol parameters
% These lengths are set only within the two main columns
%\setlength{\columnseprule}{0.25pt}
\setlength{\premulticols}{.5pt}
\setlength{\postmulticols}{.5pt}
\setlength{\multicolsep}{.5pt}
\setlength{\columnsep}{1pt}

%\begin{center}
%     \Large{\textbf{STAT564}} \\
%\end{center}

\section{565 mid-term}
\subsection{model}
$y_{ij}=\mu+\tau_{i}+\varepsilon_{ij}$, for $\varepsilon_{ij}\sim iid N(0,\sigma^2),i=1,2,…,a,j=1,2,…,n$, $\sum_{i=1}^a\tau_i=0$
Random effects: $\tau_{i}\sim iid N(0,\sigma_\tau^2)$,$\tau_{i}$ and $\varepsilon_{ij}$ indep

$y_{ij}=(\mu+\tau_{i}+\beta_j)+\varepsilon_{ij}$, for $\varepsilon_{ij}\sim iid N(0,\sigma^2),i=1,2,…,a,j=1,2,…,b$

Fixed effects: $\sum_{i=1}^a\tau_i=0, \sum_{j=1}^b\beta_j=0$
Random effects: $\beta_{j}\sim iid N(0,\sigma_\beta^2)$

Graeco-Latin square: $y_{ijkl}=\mu+\theta_i+\tau_j+\omega_k+\psi_l+\varepsilon_{ijkl}$;$i,j,k,l=1,2,..,p$

BIBD: $y_{ij}=(\mu+\tau_{i}+\beta_j)+\varepsilon_{ij}$;$i=1,2,…,a,j=1,2,…,b$;$N=kb=ra,\lambda=\frac{r(k-1)}{a-1}$

\subsubsection{least square and normal equation}
CRD:$SSE=\sum_{i=1}^a\sum_{j=1}^n(y_{ij}-\mu-\tau_i)^2$  
$\left.\frac{\partial SSE}{\partial\mu}\right|_{\hat\mu,\hat\tau_i}=2\sum_{i=1}^a\sum_{j=1}^n(y_{ij}-\hat\mu-\hat\tau_i)(-1)=0$
$y_{..}=an\hat\mu+n\sum_{i=1}^a\hat\tau_i$  
$\left.\frac{\partial SSE}{\partial\tau_i}\right|_{\hat\mu,\hat\tau_i}=2\sum_{j=1}^n(y_{ij}-\hat\mu-\hat\tau_i)(-1)=0$
$y_{i.}=n\hat\mu+n\hat\tau_i$

RCBD: $SSE=\sum_{i=1}^a\sum_{j=1}^b(y_{ij}-\mu-\tau_i-\beta_j)^2$

$\left.\frac{\partial SSE}{\partial\mu}\right|_{\hat\mu,\hat\tau_i,\hat\beta_j}=2\sum_{i=1}^a\sum_{j=1}^b(y_{ij}-\hat\mu-\hat\tau_i-\hat\beta_j)(-1)=0$    
$\left.\frac{\partial SSE}{\partial\tau_i}\right|_{\hat\mu,\hat\tau_i,\hat\beta_j}=2\sum_{j=1}^b(y_{ij}-\hat\mu-\hat\tau_i-\hat\beta_j)(-1)=0$  
$\left.\frac{\partial SSE}{\partial\beta_j}\right|_{\hat\mu,\hat\tau_i,\hat\beta_j}=2\sum_{i=1}^a(y_{ij}-\hat\mu-\hat\tau_i-\hat\beta_j)(-1)=0$  

$y_{..}=ab\hat\mu+b\sum_{i=1}^a\hat\tau_i+a\sum_{j=1}^b\hat\beta_j$

$y_{i.}=b\hat\mu+b\hat\tau_i+\sum_{j=1}^b\hat\beta_j$  

$y_{.j}=a\hat\mu+\sum_{i=1}^a\hat\tau_i+a\hat\beta_j$

\subsection{hypothesis test}
\begin{tabular}{ l|l|l }
model  &H0&H1\\
FT-CRD & $\mu_1=\mu_2=..=\mu_a$& at least two of $\mu_a$ are different\\
RT-CRD & $\sigma_{\tau}^2=0$& $\sigma_{\tau}^2>0$\\
FB-RCBD& $\mu_1=\mu_2=..=\mu_a$& at least two of $\mu_a$ are different\\
 -Block& $\beta_1=\beta_2=..=\beta_j=0$& at least one of $\beta_j\neq 0$\\
RB-RCBD& $\sigma_{\beta}^2=0$& $\sigma_{\beta}^2>0$\\
Contrast& $\Gamma=\sum_{i=1}^ac_i\mu_i=0$&$\Gamma=\sum_{i=1}^ac_i\mu_i\neq0$\\
LSD    & $\mu_1=\mu_2=..=\mu_p$& at least two of $\mu_p$ are different\\
BIBD   & $\mu_1=\mu_2=..=\mu_a$& at least two of $\mu_a$ are different\\
\end{tabular}

\subsubsection{ANOVA}
\begin{tabular}{l|l|l|l|l|}
    & SS   &      df     & MS  & F    \\
$SS_{Trt}$&$n\sum^a_{i=1}(\bar y_{i.}-\bar y_{..})^2$&$a-1$&$\frac{SS_{Trt}}{a-1}$&$\frac{MS_{Trt}}{MS_E}$\\
$SS_E$    &$\sum^a_{i=1}\sum^n_{j=1}(y_{ij} - \bar y_{i.})^2$     &$a(n-1)$& $\frac{SS_E}{N-a}$  \\
$SS_T$    &$\sum^a_{i=1}\sum^n_{j=1}(y_{ij}-\bar y_{..})^2$&$an-1$\\
\hline
$SS_{Trt}$&$b\sum^a_{i=1}(\bar y_{i.}-\bar y_{..})^2$&$a-1$&$\frac{SS_{Trt}}{a-1}$&$\frac{MS_{Trt}}{MS_E}$\\
$SS_{Blk}$&$a\sum^b_{j=1}(\bar y_{.j}-\bar y_{..})^2$&$b-1$&$\frac{SS_{Blk}}{b-1}$&$\frac{MS_{Blk}}{MS_E}$\\
$SS_E$    &$SS_T-SS_{Trt}-SS_{Blk}$ &$(a-1)(b-1)$& $\frac{SS_E}{df_E}$&\\
$SS_T$    &$\sum^a_{i=1}\sum^b_{j=1}(y_{ij}-\bar y_{..})^2$&$ab-1$\\
\hline
\end{tabular}

[f.]$SS_{Trt}=\frac1n\sum^a_{i=1}y_{i.}^2-\frac{y_{..}^2}N$

[r.]$SS_{Trt}=\frac1b\sum^a_{i=1}y_{i.}^2-\frac{y_{..}^2}N$
$SS_{Blk}=\frac1a\sum^b_{j=1}y_{.j}^2-\frac{y_{..}^2}N$ 
$SSE=\sum^a_{i=1}\sum^b_{j=1}(y_{ij}-\bar y_{i.}-\bar y_{.j}+\bar y_{..})^2$

$SS_T=\sum^a_{i=1}\sum^b_{j=1}y_{ij}^2-\frac{y_{..}^2}N$, $S^2_i=\frac{\sum_{j=1}^n(y_{ij}-\bar y_{i.})^2}{n-1}$

\begin{tabular}{l|l|l|}
LSD& SS   &      df\\
$SS_{Trt1}$&$p\sum^p_{i=1}(\bar y_{i..}-\bar y_{...})^2$&$p-1$\\
$SS_{Row}$&$p\sum^p_{j=1}(\bar y_{.j.}-\bar y_{...})^2$&$p-1$\\
$SS_{Col}$&$p\sum^p_{k=1}(\bar y_{..k}-\bar y_{...})^2$&$p-1$\\
$SS_E$    &$SS_T-SS_{.}$ &$(p-1)(p-2)$\\
$SS_T$    &$\sum^p_{i=1}\sum^p_{j=1}\sum^p_{k=1}(y_{ijk}-\bar y_{..})^2$&$p^2-1$\\ \hline
\end{tabular}

\begin{tabular}{l|l|l|l|}
df  & Case1 & Case2 & Case3 \\
$SS_{Trt}$&$p-1$&$p-1$&$p-1$\\
$SS_{Row}$&$p-1$&$n(p-1)$&$n(p-1)$\\
$SS_{Col}$&$p-1$&$p-1$&$n(p-1)$\\
$SS_{Rep}$&$n-1$&$n-1$&$n-1$\\
$SS_E$    &$(p-1)(np+n-3)$&$(p-1)(np-2)$&$(p-1)(np-n-1)$\\
$SS_T$    & $np^2-1$ & $np^2-1$ & $np^2-1$\\ \hline
\end{tabular}

\begin{tabular}{l|l|l|}
Graeco-LSD& SS   &      df\\
$SS_{Trt1}$&$b\sum^a_{i=1}(\bar y_{i.}-\bar y_{..})^2$&$p-1$\\
$SS_{Trt2}$&$b\sum^a_{i=1}(\bar y_{i.}-\bar y_{..})^2$&$p-1$\\
$SS_{Row}$&$a\sum^b_{j=1}(\bar y_{.j}-\bar y_{..})^2$&$p-1$\\
$SS_{Col}$&$a\sum^b_{j=1}(\bar y_{.j}-\bar y_{..})^2$&$p-1$\\
$SS_E$    &$SS_T-SS_{.}$ &$(p-1)(p-3)$\\
$SS_T$    &$\sum^p_{i=1}\sum^p_{j=1}(y_{ijkl}-\bar y_{..})^2$&$p^2-1$\\ \hline
\end{tabular}

\begin{tabular}{l|l|l|}
BIBD  & SS   &      df\\
$SS_{Trt}$&$\frac{k}{\lambda a}\sum^a_{i=1}Q_i^2=\frac{k}{\lambda a}\sum^a_{i=1}(y_{i.}-\sum^b_{j=1}n_{ij}\bar y_{.j})^2$&$a-1$\\
$SS_{Blk}$&$a\sum^b_{j=1}(\bar y_{.j}-\bar y_{..})^2$&$b-1$\\
$SS_E$    &$SS_T-SS_{Trt(adj)}-SS_{Blk}$ &$N-a-b+1)$\\
$SS_T$    &$\sum^a_{i=1}\sum^b_{j=1}(y_{ij}-\bar y_{..})^2$&$N-1$\\
\hline
\end{tabular}

\subsubsection{distribution}
\begin{tabular}{l|l|l|l|l|l}
  &$y_{ij}$ & $\bar y_{i.}$ & $\frac{y_{i.}-\mu_i}{\frac{\sigma}{\sqrt{n}}}$&$\bar y_{i.}-\bar y_{j.}$& $\frac{\bar y_{i.}-\bar y_{j.}-(\mu_i-\mu_j)}{\frac{2\sigma}{\sqrt{n}}}$\\
N &$(\mu+\tau_i,\sigma^2)$ & $(\mu+\tau_i,\frac{\sigma^2}n)$ & $(0,1)$&$(\mu_i-\mu_j,\frac{2\sigma^2}n)$ & $(0,1)$\\\hline
\end{tabular}

\begin{tabular}{l|l|l|l}
$t_{df_E}$&$\frac{\frac{y_{i.}-\mu_i}{\frac{\sigma}{\sqrt{n}}}}{\sqrt{\frac{SS_E}{\sigma^2(N-a)}}}=\frac{y_{i.}-\mu_i}{\sqrt{\frac{SS_E}{n(df_E)}}}=\frac{y_{i.}-\mu_i}{\sqrt{\frac{MS_E}n}}$ & $\frac{\bar y_{i.}-\bar y_{j.}-(\mu_i-\mu_j)}{\sqrt{\frac{2MS_E}n}}$&$\frac{C}{\sqrt{\widehat{Var(C)}}}$\\\hline
\end{tabular}

\begin{tabular}{l|l|l|l|l}
$\chi^2$ & $\frac{SS_E}{\sigma^2}$ &$\frac{SS_{Trt}}{\sigma^2}$ &$\frac{SS_{Blk}}{\sigma^2}$ &$SS_{C}$\\
df       & $E$ & $Trt$ & $Blk$ & $1$
\end{tabular}

\begin{tabular}{l|l|l|l}
F & $\frac{MS_{Trt}}{MS_{E}}$&$\frac{(MS_{Blk}}{MS_{E}}$&$\frac{(\sum_{i=1}^ac_i\bar y_{i.})^2}{\frac{MS_{E}}n\sum_{i=1}^ac_i^2}$\\
df& $(Trt,E)$&$(Blk,E)$&$(C=1,E)$\\
\end{tabular}




\subsubsection{contrast}

$\Gamma=\sum_{i=1}^ac_i\mu_i$,$C=\sum_{i=1}^ac_i\bar y_i$;$\sum_{i=1}^ac_i=0$;Orthogonal $\sum_{i=1}^ac_id_i=0$

$SS_C=\frac{(\sum_{i=1}^ac_i\bar y_i)^2}{\frac{1}n\sum_{i=1}^ac_i^2}$,$\sum_1^{a-1} SS_C=SS_{Trt}$

\subsubsection{CI}
\begin{tabular}{l|l|l}
        CI   & balanced & unbalanced \\
$\mu_i$      &$\bar y_{i.}\pm t_{\frac{\alpha}2}\sqrt{\frac{MS_E}{n}}$&$\bar y_{i.}\pm t_{\frac{\alpha}2}\sqrt{\frac{MS_E}{n_i}}$\\
$\mu_i-\mu_j$&$\bar y_{i.}-\bar y_{j.}\pm t_{\frac{\alpha}2}\sqrt{\frac{2MS_E}{n}}$&$\bar y_{i.}-\bar y_{j.}\pm t_{\frac{\alpha}2}\sqrt{MS_E(\frac{1}{n_i}+\frac{1}{n_j})}$\\
$\Gamma$&$\sum_{i=1}^ac_i\bar y_i\pm t_{\frac{\alpha}2}\sqrt{\frac{MS_{E}}n\sum_{i=1}^ac_i^2}$&\\
\end{tabular}


\subsubsection{expectation and variance}


$y_{..}=\sum^a_{i=1}(y_{i.}=\sum^n_{j=1}y_{ij})$,$\mu=\frac{\sum_{i=1}^a\mu_i}{a}$

$\bar y_{..}=\frac{1}N\left[y_{..}=\sum^a_{i=1}(y_{i.}=\sum^n_{j=1}y_{ij})\right]=\frac{1}a\sum^a_{i=1}\left[\bar y_{i.}=\frac{1}n(y_{i.}=\sum^n_{j=1}y_{ij})\right]$

\begin{tabular}{l|l|l|l|l|l}
     &$y_{ij}$  &$\bar y_{..}$&$\bar y_{i.}$&$\bar y_{.j}$& $C$\\
     &          &$\frac{\sum^a_{i=1}\sum^n_{j=1}y_{ij}}N$ & $\frac{\sum^n_{j=1}y_{ij}}n$ & $\frac{\sum^a_{i=1}y_{ij}}a$ & $\sum^{a}_{i=1}c_i\bar y_{i.}$\\
E[f.]  &  $\mu+\tau_i+\beta_j$   &  $\mu$      & $\mu+\tau_i$ &$\mu+\beta_j$ & $\sum^{a}_{i=1}c_i\mu_{i}$\\
V[f.]  &$\sigma^2$&$\frac{\sigma^2}{na}$&$\frac{\sigma^2}{n}$&$\frac{\sigma^2}{a}$ & $\frac{\sigma^2}n\sum^{a}_{i=1}c_i^2$\\\hline
E[r.]  &  $\mu$   &  $\mu$      &$\mu$ & $\mu$  \\
V[r.]  &$\sigma^2+\sigma_\tau^2$&$\frac{\sigma_\tau^2}{a}+\frac{\sigma^2}{na}$&$\frac{\sigma^2}{n}+\sigma_\tau^2$&$\frac{\sigma^2}{a}+\sigma_\beta^2$\\
\hline
\end{tabular}

\begin{tabular}{l|l|l|l|l}
     &$MS_{E}$  & $MS_{Trt}$ & $MS_{Trt}$ & $MS_{Blk}$ \\
E[f.]&$\sigma^2$& $\sigma^2+\frac{n}{a-1}\sum_{i=1}^a\tau_i^2$& $\sigma^2+\frac{b}{a-1}\sum_{i=1}^a\tau_i^2$&$\sigma^2+\frac{a}{b-1}\sum_{j=1}^b\beta_j^2$\\
E[r.]&$\sigma^2$& $\sigma^2+n\tau_i^2$& $\sigma^2+b\tau_i^2$ & $\sigma^2+a\beta_j^2$\\
\hline
\end{tabular}

\begin{tabular}{l|l|l|l|l|l}
&$\hat\sigma^2$&$\hat\sigma_{Trt}^2$&$\hat\sigma_{Blk}^2$&$\widehat{Var(\bar y_{i.})}$&$\widehat{Var(\bar y_{.j})}$\\
f.&$MSE$& & &$\frac{MS_{E}}{n}$& $\frac{MS_{E}}{a}$\\
r.&$MSE$&$\frac{MS_{Trt}-MS_{E}}{n}$&$\frac{MS_{Blk}-MS_{E}}{a}$&$\frac{MS_{Trt}}{n}$&$\frac{MS_{Trt}}{a}$\\
\end{tabular}

\begin{tabular}{l|l|l|l|l|l}
$\hat\mu$&$\hat\mu_i$&$\hat\tau_i$&$\hat\beta_j$&$\hat y_{ij}$&$\hat\varepsilon_{ij}$\\
$\bar y_{..}$&$\bar y_{i.}$&$\bar y_{i.}-\bar y_{..}$&$\bar y_{.j}-\bar y_{..}$&$\bar y_{i.}+\bar y_{.j}-\bar y_{..}$&$\bar y_{ij}-\bar y_{..}$\\
$\frac1{an}y_{..}-\frac1{a}\sum_{i=1}^a\hat\tau_i$& & $\frac1{a}y_{i.}-\hat\mu$\\
\hline
\end{tabular}

\begin{tabular}{l|l|l|l|l|l}
FT- &CRD & E & Var[]\\
$y_{ij}-\bar y_{i.}$ & $\varepsilon_{ij}-\frac{\sum_{j=1}^n\varepsilon_{ij}}n$ & $0$ & $\frac{n-1}n\sigma^2$\\
$\bar y_{i.}-\bar y_{..}$ & $\tau_{i}+\frac{\sum_{j=1}^n\varepsilon_{ij}}n-\frac{\sum_{i=1}^a\sum_{j=1}^n\varepsilon_{ij}}{an}$ & $\tau_i$ & $\frac{(a-1)\sigma^2}{an}$\\
\hline
RT- &CRD & E & Var[]\\
$y_{ij}-\bar y_{i.}$ & $\varepsilon_{ij}-\frac{\sum_{j=1}^n\varepsilon_{ij}}n$ & $0$ & $\frac{n-1}n\sigma^2$\\
$\bar y_{i.}-\bar y_{..}$ & $\tau_{i}-\frac{\sum_{i=1}^a\tau_{i}}{a}+\frac{\sum_{j=1}^n\varepsilon_{ij}}n-\frac{\sum_{i=1}^a\sum_{j=1}^n\varepsilon_{ij}}{an}$ & $0$ & $\frac{(a-1)(n\sigma_{\tau}^2+\sigma^2)}{an}$\\
\hline
F- &RCBD & E & Var[]\\
$y_{ij}-\bar y_{i.}$ & $\beta_{j}+\varepsilon_{ij}-\frac{\sum_{j=1}^b\varepsilon_{ij}}b$ & $\beta_j$ & $\frac{(b-1)\sigma^2}b$\\
$\bar y_{i.}-\bar y_{..}$ & $\tau_{i}+\frac{\sum_{j=1}^b\varepsilon_{ij}}b-\frac{\sum_{i=1}^a\sum_{j=1}^b\varepsilon_{ij}}{ab}$ & $\tau_i$ & $\frac{(a-1)\sigma^2}{ab}$\\
$y_{ij}-\bar y_{.j}$ & $\tau_{i}+\varepsilon_{ij}-\frac{\sum_{i=1}^a\varepsilon_{ij}}a$ & $\tau_i$ & $\frac{(a-1)\sigma^2}a$\\
$\bar y_{.j}-\bar y_{..}$ & $\beta_{j}+\frac{\sum_{i=1}^a\varepsilon_{ij}}a-\frac{\sum_{i=1}^a\sum_{j=1}^b\varepsilon_{ij}}{ab}$ & $\beta_j$ & $\frac{(b-1)\sigma^2}{ab}$\\
\hline
R- &RCBD & E & Var[]\\
$y_{ij}-\bar y_{i.}$ & $\beta_{j}-\frac{\sum_{j=1}^b\beta_{j}}b+\varepsilon_{ij}-\frac{\sum_{j=1}^b\varepsilon_{ij}}b$ & $0$ & $\frac{(b-1)(\sigma_{\beta}^2+\sigma^2)}b$\\
$\bar y_{i.}-\bar y_{..}$ & $\tau_{i}+\frac{\sum_{j=1}^b\varepsilon_{ij}}b-\frac{\sum_{i=1}^a\sum_{j=1}^b\varepsilon_{ij}}{ab}$ & $\tau_i$ & $\frac{(a-1)\sigma^2}{ab}$\\
$y_{ij}-\bar y_{.j}$ & $\tau_{i}+\varepsilon_{ij}-\frac{\sum_{i=1}^a\varepsilon_{ij}}a$ & $\tau_i$ & $\frac{(a-1)\sigma^2}a$\\
$\bar y_{.j}-\bar y_{..}$ & $\beta_j-\frac{\sum_{j=1}^b\beta_j}{b}+\frac{\sum_{i=1}^a\varepsilon_{ij}}a-\frac{\sum_{i=1}^a\sum_{j=1}^b\varepsilon_{ij}}{ab}$ & $0$ & $\frac{(b-1)(a\sigma_{\beta}^2+\sigma^2)}{ab}$\\
\end{tabular}

$y_{ij}-\bar y_{i.}-\bar y_{.j}+\bar y_{..}=\varepsilon_{ij}-\frac{\sum_{i=1}^a\varepsilon_{ij}}a-\frac{\sum_{j=1}^b\varepsilon_{ij}}b+\frac{\sum_{i=1}^a\sum_{j=1}^b\varepsilon_{ij}}{ab}$

$E[]=0, Var=\frac{(a-1)(b-1)\sigma^2}{ab}$


\subsubsection{covariance}

R-CRD: $Cov(y_{ij},y_{kl})=\begin{cases}0,i\neq k; \sigma_{\tau}^2,i=k,j\neq l ; \sigma^2+\sigma_{\tau}^2,i=k,j=l\end{cases}$

\begin{tabular}{l|l|l|l|l}
&$\varepsilon_{ij}$&$\sum_{i=1}^a\varepsilon_{ij}$&$\sum_{j=1}^b\varepsilon_{ij}$&$\sum_{i=1}^a\sum_{j=1}^b\varepsilon_{ij}$\\
$\varepsilon_{ij}$&$\sigma^2$&$\sigma^2$&$\sigma^2$&$\sigma^2$\\
$\sum_{i=1}^a\varepsilon_{ij}$&&$a\sigma^2$&$\sigma^2$&$a\sigma^2$\\
$\sum_{j=1}^b\varepsilon_{ij}$&&&$b\sigma^2$&$b\sigma^2$\\
$\sum_{i=1}^a\sum_{j=1}^b\varepsilon_{ij}$&&&&$ab\sigma^2$
\end{tabular}

\end{multicols}

$Cov[\varepsilon_{ij},\varepsilon_{ij}]=Cov[\sum_{i1}^a\varepsilon_{ij},\sum_{j=1}^b\varepsilon_{ij}]=\sigma^2$,$Cov[\tau_{i},\tau_{i}]=σ_{\tau}^2$,$Cov[\beta_{j},\beta_{j}]=σ_{\beta}^2$

$Cov[\varepsilon_{ij},\tau_{i}]=Cov[\varepsilon_{ij},\beta_{j}]=Cov[\tau_{i},\beta_{j}]=Cov[\varepsilon_{ij},\varepsilon_{ik}]=0,k\neq j$

$Cov[\varepsilon_{ij},\sum_{j=1}^n\varepsilon_{ij}]=Cov[\varepsilon_{ij},(\varepsilon_{i1}+..+\varepsilon_{ij}..+\varepsilon_{in})]=Cov[\varepsilon_{ij},\varepsilon_{i1}]+..+Cov[\varepsilon_{ij},\varepsilon_{ij}]..+Cov[\varepsilon_{ij},\varepsilon_{in}]=\sigma^2$

$Cov[\sum_{j=1}^n\varepsilon_{ij},\sum_{i=1}^a\sum_{j=1}^n\varepsilon_{ij}]=Cov[(\varepsilon_{i1}+\varepsilon_{i2}..+\varepsilon_{in}),(\varepsilon_{i1}+\varepsilon_{i2}..+\varepsilon_{in})]=Cov[\varepsilon_{i1},\varepsilon_{i1}]+Cov[\varepsilon_{i2},\varepsilon_{i2}]..+Cov[\varepsilon_{in},\varepsilon_{in}]=n\sigma^2$

$Var[y_{ij}-\bar y_{i.}]=$

FT-CRD;RT-CRD

$Var[\varepsilon_{ij}-\frac{\sum_{j=1}^n\varepsilon_{ij}}n]=$,
$Var[\varepsilon_{ij}]+\frac{\sum_{j=1}^nVar[\varepsilon_{ij}]}{n^2}-\frac{2Cov[\varepsilon_{ij},\sum_{j=1}^n\varepsilon_{ij}]}n$,
$=\sigma^2+\frac{\sigma^2}n-\frac2n\sigma^2=\frac{n-1}n\sigma^2$

FB-RCBD

$Var[\beta_{j}+\varepsilon_{ij}-\frac{\sum_{j=1}^b\varepsilon_{ij}}b]=$,
$Var[\beta_{j}]+Var[\varepsilon_{ij}]+\frac{\sum_{j=1}^bVar[\varepsilon_{ij}]}{b^2}-2Cov[\beta_{j},\varepsilon_{ij}]-\frac{2Cov[\beta_{j},\sum_{j=1}^b\varepsilon_{ij}]}b-\frac{2Cov[\varepsilon_{ij},\sum_{j=1}^b\varepsilon_{ij}]}b$,
$=0+\sigma^2+\frac{\sigma^2}b-0-0-\frac{2\sigma^2}b=\frac{(b-1)\sigma^2}b$

RB-RCBD

$Var[\beta_{j}-\frac{\sum_{j=1}^b\beta_{j}}b+\varepsilon_{ij}-\frac{\sum_{j=1}^b\varepsilon_{ij}}b]=$
$Var[\beta_{j}]+\frac{\sum_{j=1}^bVar[\beta_{j}]}{b^2}+Var[\varepsilon_{ij}]+\frac{\sum_{j=1}^bVar[\varepsilon_{ij}]}{b^2}-\frac{2Cov[\beta_{j},\sum_{j=1}^b\beta_{j}]}b+2Cov[\beta_{j},\varepsilon_{ij}]-\frac{2Cov[\beta_{j},\sum_{j=1}^b\varepsilon_{ij}]}b-\frac{2Cov[\sum_{j=1}^b\beta_{j},\varepsilon_{ij}]}b$
$+\frac{2Cov[\sum_{j=1}^b\beta_{j},\sum_{j=1}^b\varepsilon_{ij}]}{b^2}-\frac{2Cov[\varepsilon_{ij},\sum_{j=1}^b\varepsilon_{ij}]}b$
$=\sigma_{\beta}^2+\frac{\sigma_{\beta}^2}{b}-\frac{2\sigma_{\beta}^2}{b}+\sigma^2+\frac{\sigma^2}b-\frac{2\sigma^2}b=\frac{(\sigma_{\beta}^2+\sigma^2)(b-1)}b$

 ---

$Var[\bar y_{i.}-\bar y_{..}]=$

FT-CRD

$Var[\tau_{i}+\frac{\sum_{j=1}^n\varepsilon_{ij}}n-\frac{\sum_{i=1}^a\sum_{j=1}^n\varepsilon_{ij}}{an}]=$
$Var[\tau_{i}]+\frac{\sum_{j=1}^nVar[\varepsilon_{ij}]}{n^2}+\frac{\sum_{i=1}^a\sum_{j=1}^nVar[\varepsilon_{ij}]}{a^2n^2}+\frac{2Cov[\tau_{i},\sum_{j=1}^n\varepsilon_{ij}]}{n}-\frac{2Cov[\tau_{i},\sum_{i=1}^a\sum_{j=1}^n\varepsilon_{ij}]}{an}-\frac{2Cov[\sum_{j=1}^n\varepsilon_{ij},\sum_{i=1}^a\sum_{j=1}^n\varepsilon_{ij}]}{an^2}$,
$=0+\frac{\sigma^2}{n}+\frac{\sigma^2}{an}-\frac{2\sigma^2}{an}=\frac{(a-1)\sigma^2}{an}$

RT-CRD

$Var[\tau_{i}-\frac{\sum_{i=1}^a\tau_{i}}{a}+\frac{\sum_{j=1}^n\varepsilon_{ij}}n-\frac{\sum_{i=1}^a\sum_{j=1}^n\varepsilon_{ij}}{an}]=$
$Var[\tau_{i}]+\frac{\sum_{i=1}^aVar[\tau_{i}]}{a^2}+\frac{\sum_{j=1}^nVar[\varepsilon_{ij}]}{n^2}+\frac{\sum_{i=1}^a\sum_{j=1}^nVar[\varepsilon_{ij}]}{a^2n^2}-\frac{2Cov[\tau_{i},\sum_{i=1}^a\tau_{i}]}a+\frac{2Cov[\tau_{i},\sum_{j=1}^n\varepsilon_{ij}]}n-\frac{2Cov[\tau_{i},\sum_{i=1}^a\sum_{j=1}^n\varepsilon_{ij}]}{an}-\frac{2Cov[\sum_{i=1}^a\tau_{i},\sum_{j=1}^n\varepsilon_{ij}]}{an}$
$+\frac{2Cov[\sum_{i=1}^a\tau_{i},\sum_{i=1}^a\sum_{j=1}^n\varepsilon_{ij}]}{a^2n}-\frac{2Cov[\sum_{j=1}^n\varepsilon_{ij},\sum_{i=1}^a\sum_{j=1}^n\varepsilon_{ij}]}{an^2}$
$=\sigma_{\tau}^2+\frac{\sigma_{\tau}^2}{a}-\frac{2\sigma_{\tau}^2}{a}+\frac{\sigma^2}{n}+\frac{\sigma^2}{an}-\frac{2\sigma^2}{an}=\frac{(n\sigma_{\tau}^2+\sigma^2)(a-1)}{an}$

FB-RCBD;RB-RCBD

$Var[\tau_{i}+\frac{\sum_{j=1}^b\varepsilon_{ij}}b-\frac{\sum_{i=1}^a\sum_{j=1}^b\varepsilon_{ij}}{ab}]=$
$Var[\tau_{i}]+\frac{\sum_{j=1}^bVar[\varepsilon_{ij}]}{b^2}+\frac{\sum_{i=1}^a\sum_{j=1}^bVar[\varepsilon_{ij}]}{a^2b^2}+\frac{2Cov[\tau_{i},\sum_{j=1}^b\varepsilon_{ij}]}{b}-\frac{2Cov[\tau_{i},\sum_{i=1}^a\sum_{j=1}^b\varepsilon_{ij}]}{ab}-\frac{2Cov[\sum_{j=1}^b\varepsilon_{ij},\sum_{i=1}^a\sum_{j=1}^b\varepsilon_{ij}]}{ab^2}$
$=0+\frac{\sigma^2}{b}+\frac{\sigma^2}{ab}-\frac{2\sigma^2}{ab}=\frac{(a-1)\sigma^2}{ab}$

 ---

$Var[y_{ij}-\bar y_{.j}]=$

FB-RCBD; RB-RCBD

$Var[\tau_{i}+\varepsilon_{ij}-\frac{\sum_{i=1}^a\varepsilon_{ij}}a]=$
$Var[\tau_{i}]+Var[\varepsilon_{ij}]+\frac{\sum_{i=1}^aVar[\varepsilon_{ij}]}{a^2}-\frac{2Cov[\tau_{i},\varepsilon_{ij}]}a-\frac{2Cov[\tau_{i},\sum_{i=1}^a\varepsilon_{ij}]}a-\frac{2Cov[\varepsilon_{ij},\sum_{i=1}^a\varepsilon_{ij}]}a$
$=0+\sigma^2+\frac{\sigma^2}a-\frac{2\sigma^2}a=\frac{(a-1)\sigma^2}a$

 ---

$Var[\bar y_{.j}-\bar y_{..}]=$

FB-RCBD

$Var[\beta_{j}+\frac{\sum_{i=1}^a\varepsilon_{ij}}a-\frac{\sum_{i=1}^a\sum_{j=1}^b\varepsilon_{ij}}{ab}]=$
$Var[\beta_{j}]+\frac{\sum_{i=1}^aVar[\varepsilon_{ij}]}{a^2}+\frac{\sum_{i=1}^a\sum_{j=1}^bVar[\varepsilon_{ij}]}{a^2b^2}+\frac{2Cov[\beta_{j},\sum_{i=1}^a\varepsilon_{ij}]}{a}-\frac{2Cov[\beta_{j},\sum_{i=1}^a\sum_{j=1}^b\varepsilon_{ij}]}{ab}-\frac{2Cov[\sum_{i=1}^a\varepsilon_{ij},\sum_{i=1}^a\sum_{j=1}^b\varepsilon_{ij}]}{a^2b}$
$=0+\frac{\sigma^2}{a}+\frac{\sigma^2}{ab}-\frac{2\sigma^2}{ab}=\frac{(b-1)\sigma^2}{ab}$

RB-RCBD

$Var[\beta_{j}-\frac{\sum_{j=1}^b\beta_{j}}{b}+\frac{\sum_{i=1}^a\varepsilon_{ij}}a-\frac{\sum_{i=1}^a\sum_{j=1}^b\varepsilon_{ij}}{ab}]=$,
$Var[\beta_{j}]+\frac{\sum_{j=1}^bVar[\beta_{j}]}{b^2}+\frac{\sum_{i=1}^aVar[\varepsilon_{ij}]}{a^2}+\frac{\sum_{i=1}^a\sum_{j=1}^bVar[\varepsilon_{ij}]}{a^2b^2}-\frac{2Cov[\beta_{j},\sum_{j=1}^b\beta_{j}]}b+\frac{2Cov[\beta_{j},\sum_{i=1}^a\varepsilon_{ij}]}a-\frac{2Cov[\beta_{j},\sum_{i=1}^a\sum_{j=1}^b\varepsilon_{ij}]}{ab}-\frac{2Cov[\sum_{j=1}^b\beta_{j},\sum_{i=1}^a\varepsilon_{ij}]}{ab}$
$+\frac{2Cov[\sum_{j=1}^b\beta_{j},\sum_{i=1}^a\sum_{j=1}^b\varepsilon_{ij}]}{ab^2}-\frac{2Cov[\sum_{i=1}^a\varepsilon_{ij},\sum_{i=1}^a\sum_{j=1}^b\varepsilon_{ij}]}{a^2b}$
$=\sigma_{\beta}^2+\frac{\sigma_{\beta}^2}{b}-\frac{2\sigma_{\beta}^2}{b}+\frac{\sigma^2}{a}+\frac{\sigma^2}{ab}-\frac{2\sigma^2}{ab}=\frac{(a\sigma_{\beta}^2+\sigma^2)(b-1)}{ab}$

 ---

$Var[y_{ij}-\bar y_{i.}-\bar y_{.j}+\bar y_{..}]=$
FB-RCBD

$Var[\varepsilon_{ij}-\frac1a\sum_{i=1}^a\varepsilon_{ij}-\frac1b\sum_{j=1}^b\varepsilon_{ij}+\frac1{ab}\sum_{i=1}^a\sum_{j=1}^b\varepsilon_{ij}]=$
$Var[\varepsilon_{ij}]+\frac{\sum_{i=1}^aVar[\varepsilon_{ij}]}{a^2}+\frac{\sum_{j=1}^bVar[\varepsilon_{ij}]}{b^2}+\frac{\sum_{i=1}^a\sum_{j=1}^bVar[\varepsilon_{ij}]}{a^2b^2}-\frac{2Cov[\varepsilon_{ij},\sum_{i=1}^a\varepsilon_{ij}]}{a}-\frac{2Cov[\varepsilon_{ij},\sum_{j=1}^b\varepsilon_{ij}]}{b}+\frac{2Cov[\varepsilon_{ij},\sum_{i=1}^a\sum_{j=1}^b\varepsilon_{ij}]}{ab}+\frac{2Cov[\sum_{i=1}^a\varepsilon_{ij},\sum_{j=1}^b\varepsilon_{ij}]}{ab}$
$-\frac{2Cov[\sum_{i=1}^a\varepsilon_{ij},\sum_{i=1}^a\sum_{j=1}^b\varepsilon_{ij}]}{a^2b}-\frac{2Cov[\sum_{j=1}^b\varepsilon_{ij},\sum_{i=1}^a\sum_{j=1}^b\varepsilon_{ij}]}{ab^2}$
$=\sigma^2+\frac{\sigma^2}{a}+\frac{\sigma^2}{b}+\frac{\sigma^2}{ab}-\frac{2\sigma^2}{a}-\frac{2\sigma^2}{b}+\frac{2\sigma^2}{ab}+\frac{2\sigma^2}{ab}-\frac{2\sigma^2}{ab}-\frac{2\sigma^2}{ab}=\frac{(ab-a-b+1)\sigma^2}{ab}$



\end{document}
